ChoiceAlgebra/theories/ChoiceAlgebra.v
@@ -1,4 +1,4 @@
-From ChoiceAlgebra Require Import Prelude Substitution Resource.
+From ChoiceAlgebra Require Import Prelude Store Resource.
 
 (** * Choice Algebra  (Definitions 1.6)
 
