ChoiceAlgebra/theories/Store.v
@@ -1,0 +1,170 @@
+From ChoiceAlgebra Require Import Prelude MapFilterDom.
+
+(** * Stores  (Definition 1.1)
+
+    A store is a finite partial map from variables to values.
+    We use stdpp's [gmap] which requires [Countable Var] and [EqDecision Value].
+
+    We call these "stores" rather than "substitutions" to avoid name clashes
+    with the locally-nameless substitution machinery in CoreLang. *)
+
+Section Store.
+
+Context `{Countable Var} `{EqDecision Value} `{Inhabited Value}.
+
+(** ** Basic type *)
+
+Definition Store : Type := gmap Var Value.
+
+(** ** Compatibility and restriction *)
+
+(** Two stores are compatible when they agree on their common domain. *)
+Definition store_compat (s1 s2 : Store) : Prop :=
+  ∀ x v1 v2, s1 !! x = Some v1 → s2 !! x = Some v2 → v1 = v2.
+
+(** Restriction of a store to a finite set of variables. *)
+Definition store_restrict (s : Store) (X : gset Var) : Store :=
+  filter (λ '(k, _), k ∈ X) s.
+
+(** ** Lemmas *)
+
+Lemma store_compat_refl s : store_compat s s.
+Proof.
+  unfold store_compat. intros x v1 v2 H1 H2. hauto.
+Qed.
+
+Lemma store_compat_sym s1 s2 :
+  store_compat s1 s2 → store_compat s2 s1.
+Proof. unfold store_compat. intros Hc x v1 v2 H1 H2. hauto. Qed.
+
+Lemma store_compat_union s1 s2 :
+  store_compat s1 s2 →
+  store_compat (s1 ∪ s2) (s1 ∪ s2).
+Proof. unfold store_compat. intros Hc x v1 v2 H1 H2. hauto. Qed.
+
+Lemma store_restrict_dom s X :
+  dom (store_restrict s X) = dom s ∩ X.
+Proof.
+  unfold store_restrict. apply dom_gmap_filter_key_in_pair.
+Qed.
+
+Lemma store_restrict_idemp s X :
+  dom s ⊆ X → store_restrict s X = s.
+Proof.
+  unfold store_restrict. intros Hsub. apply map_filter_id.
+  intros i x Hx. apply elem_of_dom_2 in Hx. set_solver.
+Qed.
+
+Lemma store_restrict_restrict s X Y :
+  store_restrict (store_restrict s X) Y = store_restrict s (X ∩ Y).
+Proof.
+  unfold store_restrict.
+  setoid_rewrite map_filter_filter.
+  apply map_filter_ext.
+  intros i x Hx. apply elem_of_dom_2 in Hx. set_solver.
+Qed.
+
+Lemma store_union_dom s1 s2 :
+  store_compat s1 s2 →
+  dom (s1 ∪ s2) = dom s1 ∪ dom s2.
+Proof.
+  intros Hcomp. setoid_rewrite dom_union_L. auto.
+Qed.
+
+Lemma store_restrict_induce_disjoint s1 s2 :
+  s1 ##ₘ (store_restrict s2 (dom s2 ∖ dom s1)) ∧
+  s1 ∪ s2 = s1 ∪ (store_restrict s2 (dom s2 ∖ dom s1)).
+Proof.
+  pose (s2' := store_restrict s2 (dom s2 ∖ dom s1)).
+  split.
+  - rewrite map_disjoint_alt. intros i.
+    destruct (decide (i ∈ dom s1)).
+    + right.
+      apply map_lookup_filter_None_2. right.
+      intros x Hx Hi%elem_of_difference.
+      destruct Hi as [_ Hi']. by apply Hi'.
+    + left. by apply not_elem_of_dom.
+  - apply map_eq. intros i.
+    destruct (s1 !! i) as [x|] eqn:E1.
+    + rewrite (lookup_union_l' s1 s2 i) by (by exists x; exact E1).
+      rewrite (lookup_union_l' s1 s2' i) by (by exists x; exact E1).
+      reflexivity.
+    + rewrite (lookup_union_r s1 s2 i) by done.
+      rewrite (lookup_union_r s1 s2' i) by done.
+      destruct (s2 !! i) as [y|] eqn:E2.
+      * etrans.
+        -- exact E2.
+        -- symmetry. unfold s2', store_restrict.
+           apply map_lookup_filter_Some_2; first exact E2.
+           apply elem_of_difference. split.
+           ++ by apply elem_of_dom; exists y.
+           ++ by apply not_elem_of_dom.
+      * apply eq_trans with (@None Value); first exact E2.
+        symmetry. unfold s2', store_restrict.
+        apply map_lookup_filter_None. left. exact E2.
+Qed.
+
+Lemma store_restrict_union s1 s2 X :
+  store_compat s1 s2 →
+  store_restrict (s1 ∪ s2) X = store_restrict s1 X ∪ store_restrict s2 X.
+Proof.
+  intros Hcomp.
+  unfold store_restrict.
+  setoid_rewrite gmap_filter_key_pair.
+  apply map_eq. intros i.
+  rewrite option_eq. intros x.
+  setoid_rewrite map_lookup_filter_Some.
+  setoid_rewrite lookup_union_Some_raw.
+  setoid_rewrite map_lookup_filter_Some.
+  setoid_rewrite map_lookup_filter_None.
+  simpl. split.
+  - intros [[H1|[H1 H2]] HP].
+    + left. eauto.
+    + right. split. { left. exact H1. } eauto.
+  - intros [[H1 HP]|[[H1|H1] [H2 HP]]].
+    + split. { left. exact H1. } exact HP.
+    + split. { right. eauto. } exact HP.
+    + destruct (s1 !! i) as [y|] eqn:Ey.
+      * exfalso. exact (H1 y Ey HP).
+      * split. { right. eauto. } exact HP.
+Qed.
+
+Lemma store_restrict_lookup_some s X x y :
+  store_restrict s X !! x = Some y → x ∈ X ∧ s !! x = Some y.
+Proof.
+  unfold store_restrict. intro Hlookup.
+  apply map_lookup_filter_Some in Hlookup.
+  destruct Hlookup as [H1 H2]. split; [exact H2 | exact H1].
+Qed.
+
+Lemma store_compat_restrict s1 s2 X :
+  store_compat s1 s2 → store_compat (store_restrict s1 X) (store_restrict s2 X).
+Proof.
+  unfold store_compat. intros Hcomp x y z H2 H3.
+  apply store_restrict_lookup_some in H2.
+  apply store_restrict_lookup_some in H3.
+  hauto.
+Qed.
+
+Lemma store_compat_restrict_eq s1 s2 :
+  store_compat s1 s2 →
+  dom s1 ⊆ dom s2 →
+  store_restrict s2 (dom s1) = s1.
+Proof.
+  unfold store_compat. intros Hcomp Hsub.
+  unfold store_restrict.
+  apply map_eq. intros i.
+  destruct (decide (i ∈ dom s1)) as [Hin|Hnin].
+  - assert (i ∈ dom s2) as Hin2 by set_solver.
+    pose (lookup_lookup_total_dom _ _ Hin) as Hlookup1.
+    pose (lookup_lookup_total_dom _ _ Hin2) as Hlookup2.
+    rewrite Hlookup1.
+    rewrite map_lookup_filter_Some.
+    split; eauto.
+    rewrite (Hcomp i (s1 !!! i) (s2 !!! i)); eauto.
+  - assert (s1 !! i = None) as Hnone by (by apply not_elem_of_dom).
+    setoid_rewrite Hnone.
+    rewrite map_lookup_filter_None. hauto.
+Qed.
+
+End Store.
